VCVio/OracleComp/SimSemantics/UntilSwap.lean
@@ -17,16 +17,17 @@ This can be usefull when sequencing two computations when you want to avoid expl
 the size of the state type (as `SimOracle.append` would do) it makes it possible to use
 a sum type instead of a product type.
 
-NOTE: this could be generalized to go back and forth more generally,
-but seems unneeded until we have an actual use case.
+NOTE: This may not be workable without `MonadLift (StateT σ m) (StateT (σ ⊕ τ) m)`.
 -/
 
 open OracleSpec OracleComp Sum Prod
 
+universe u v w
+
 namespace SimOracle
 
-variable {ι₁ ι₂ ι : Type} {spec₁ : OracleSpec ι₁} {spec₂ : OracleSpec ι₂}
-    {spec : OracleSpec ι} {σ₁ σ₂ α β γ : Type}
+variable {ι₁ ι₂ ι : Type*} {spec₁ : OracleSpec ι₁} {spec₂ : OracleSpec ι₂}
+    {spec : OracleSpec ι} {σ₁ σ₂ : Type u} {α β γ : Type v}
 
 /-- Given two simulation oracles `so` and `so'` with the same target `spec : OracleSpec ι`,
 construct a simulation oracle that uses `so` for queries to the first and then starts using `so'`
@@ -36,33 +37,33 @@ after recieving queries to the first.
 The function `f` is used to move to the second state type after the swap.
 NOTE: `f` could eventually be an `OracleComp spec σ₂`, but no clear use case,
 maybe if this where a two way thing then it could be used for failures. -/
-def untilSwap (so : spec₁ →[σ₁]ₛₒ spec) (so' : spec₂ →[σ₂]ₛₒ spec)
-    (f : σ₁ → σ₂) : spec₁ ++ₒ spec₂ →[σ₁ ⊕ σ₂]ₛₒ spec where impl
+def untilSwap (so : SimOracle spec₁ spec σ₁) (so' : SimOracle spec₂ spec σ₂)
+    (f : σ₁ → σ₂) : SimOracle (spec₁ ++ₒ spec₂) spec (σ₁ ⊕ σ₂) where impl
   | query (inl i) t, inl s => map id inl <$> so.impl (query i t) s
   | query (inr i) t, inl s => map id inr <$> so'.impl (query i t) (f s)
   | query (inr i) t, inr s => map id inr <$> so'.impl (query i t) s
-  | _, _ => failure -- swapped back to first from second
+  | query (inl _) _, inr _ => failure -- swapped back to first from second
 
-variable (so : spec₁ →[σ₁]ₛₒ spec) (so' : spec₂ →[σ₂]ₛₒ spec) (f : σ₁ → σ₂)
+variable (so : SimOracle spec₁ spec σ₁) (so' : SimOracle spec₂ spec σ₂) (f : σ₁ → σ₂)
 
-/-- Simulating a computation using only `spec₁` bound to a computation using only `spec₂`
-(using the natural `OracleSpec.append` coercions) with `SimOracle.untilSwap so so' f`
-is the same as simulating the first with `so` and then simulating the second with `so'`,
-using the function `f` to bridge the gap between the two states. -/
-lemma simulate_untilSwap_coe_bind_coe (oa : OracleComp spec₁ α)
-    (ob : α → OracleComp spec₂ β) (s : σ₁) :
-    simulate (so.untilSwap so' f) (inl s) (↑oa >>= λ x ↦ ↑(ob x)) = (do
-      let (x, s') ← simulate so s oa
-      Prod.map id inr <$> simulate so' (f s') (ob x)) :=
-  sorry
+-- /-- Simulating a computation using only `spec₁` bound to a computation using only `spec₂`
+-- (using the natural `OracleSpec.append` coercions) with `SimOracle.untilSwap so so' f`
+-- is the same as simulating the first with `so` and then simulating the second with `so'`,
+-- using the function `f` to bridge the gap between the two states. -/
+-- lemma simulate_untilSwap_coe_bind_coe (oa : OracleComp spec₁ α)
+--     (ob : α → OracleComp spec₂ β) (s : σ₁) :
+--     simulate (untilSwap so so' f) (inl s) (↑oa >>= λ x ↦ ↑(ob x)) = (do
+--       let (x, s') ← simulate so s oa
+--       Prod.map id inr <$> simulate so' (f s') (ob x)) :=
+--   sorry
 
-/-- Version of `simulate_untilSwap_coe_bind_coe` when the final state doesn't matter. -/
-lemma simulate'_untilSwap_coe_bind_coe (oa : OracleComp spec₁ α)
-    (ob : α → OracleComp spec₂ β) (s : σ₁) :
-    simulate' (so.untilSwap so' f) (inl s) (↑oa >>= λ x ↦ ↑(ob x)) = (do
-      let (x, s') ← simulate so s oa
-      simulate' so' (f s') (ob x)) :=
-  sorry
+-- /-- Version of `simulate_untilSwap_coe_bind_coe` when the final state doesn't matter. -/
+-- lemma simulate'_untilSwap_coe_bind_coe (oa : OracleComp spec₁ α)
+--     (ob : α → OracleComp spec₂ β) (s : σ₁) :
+--     simulate' (untilSwap so so' f) (inl s) (↑oa >>= λ x ↦ ↑(ob x)) = (do
+--       let (x, s') ← simulate so s oa
+--       simulate' so' (f s') (ob x)) :=
+--   sorry
 
 
 end SimOracle
